03Debruijn/Multisubst.thy
@@ -2,26 +2,26 @@ theory Multisubst
   imports Debruijn
 begin
 
-inductive subst_pairs :: "ty list \<Rightarrow> dexpr list \<Rightarrow> bool" where
-  subp_nil [simp]: "subst_pairs [] []"
-| subp_cons [simp]: "[] \<turnstile>\<^sub>d e : t \<Longrightarrow> vald e \<Longrightarrow> subst_pairs \<Gamma> es \<Longrightarrow> subst_pairs (t # \<Gamma>) (e # es)"
+inductive tc_pairs :: "ty list \<Rightarrow> dexpr list \<Rightarrow> bool" where
+  tcp_nil [simp]: "tc_pairs [] []"
+| tcp_cons [simp]: "[] \<turnstile>\<^sub>d e : t \<Longrightarrow> vald e \<Longrightarrow> tc_pairs \<Gamma> es \<Longrightarrow> tc_pairs (t # \<Gamma>) (e # es)"
 
 primrec multisubst :: "dexpr list \<Rightarrow> dexpr \<Rightarrow> dexpr" where
   "multisubst [] e = e"
 | "multisubst (e' # es) e = multisubst es (substd 0 e' e)"
 
-lemma [simp]: "subst_pairs \<Gamma> es \<Longrightarrow> vald e \<Longrightarrow> x \<le> length \<Gamma> \<Longrightarrow> [] \<turnstile>\<^sub>d e : t \<Longrightarrow> 
-  subst_pairs (insert_at x t \<Gamma>) (insert_at x e es)"
-proof (induction \<Gamma> es arbitrary: x rule: subst_pairs.induct)
-  case (subp_cons t' e' \<Gamma> es)
+lemma [simp]: "tc_pairs \<Gamma> es \<Longrightarrow> vald e \<Longrightarrow> x \<le> length \<Gamma> \<Longrightarrow> [] \<turnstile>\<^sub>d e : t \<Longrightarrow> 
+  tc_pairs (insert_at x t \<Gamma>) (insert_at x e es)"
+proof (induction \<Gamma> es arbitrary: x rule: tc_pairs.induct)
+  case (tcp_cons t' e' \<Gamma> es)
   then show ?case by (induction x) simp_all
 qed simp_all
 
-lemma [simp]: "subst_pairs \<Gamma> es \<Longrightarrow> \<Gamma> \<turnstile>\<^sub>d e : t \<Longrightarrow> [] \<turnstile>\<^sub>d multisubst es e : t"
-proof (induction \<Gamma> es arbitrary: e rule: subst_pairs.induct)
-  case (subp_cons e' t' \<Gamma> es)
-  moreover from subp_cons have "insert_at 0 t' \<Gamma> \<turnstile>\<^sub>d e : t" by (induction \<Gamma>) simp_all
-  moreover from subp_cons have "[] \<turnstile>\<^sub>d e' : t'" by simp
+lemma [simp]: "tc_pairs \<Gamma> es \<Longrightarrow> \<Gamma> \<turnstile>\<^sub>d e : t \<Longrightarrow> [] \<turnstile>\<^sub>d multisubst es e : t"
+proof (induction \<Gamma> es arbitrary: e rule: tc_pairs.induct)
+  case (tcp_cons e' t' \<Gamma> es)
+  moreover hence "insert_at 0 t' \<Gamma> \<turnstile>\<^sub>d e : t" by (induction \<Gamma>) simp_all
+  moreover from tcp_cons have "[] \<turnstile>\<^sub>d e' : t'" by simp
   moreover hence "\<Gamma> \<turnstile>\<^sub>d e' : t'" using tc_postpend by fastforce
   ultimately show ?case by simp
 qed simp_all
@@ -43,17 +43,17 @@ lemma [simp]: "\<exists>e'. multisubst es (DLam t e) = DLam t e' \<and>
     (\<forall>e\<^sub>2. (\<forall>ee. substd 0 ee e\<^sub>2 = e\<^sub>2) \<longrightarrow> substd 0 e\<^sub>2 e' = multisubst es (substd 0 e\<^sub>2 e))"
   by (induction es arbitrary: e) simp_all
 
-lemma [simp]: "subst_pairs \<Gamma> es \<Longrightarrow> insert_at 0 t\<^sub>1 \<Gamma> \<turnstile>\<^sub>d e : t\<^sub>2 \<Longrightarrow> 
+lemma [simp]: "tc_pairs \<Gamma> es \<Longrightarrow> insert_at 0 t\<^sub>1 \<Gamma> \<turnstile>\<^sub>d e : t\<^sub>2 \<Longrightarrow> 
   \<exists>e'. multisubst es (DLam t\<^sub>1 e) = DLam t\<^sub>1 e' \<and> ([t\<^sub>1] \<turnstile>\<^sub>d e' : t\<^sub>2) \<and>
     (\<forall>e\<^sub>2. ([] \<turnstile>\<^sub>d e\<^sub>2 : t\<^sub>1) \<longrightarrow> multisubst (insert_at 0 e\<^sub>2 es) e = substd 0 e\<^sub>2 e')"
-proof (induction \<Gamma> es arbitrary: e rule: subst_pairs.induct)
-  case (subp_cons e' t \<Gamma> es)
+proof (induction \<Gamma> es arbitrary: e rule: tc_pairs.induct)
+  case (tcp_cons e' t \<Gamma> es)
   hence "[] \<turnstile>\<^sub>d e' : t" by simp
   hence "\<Gamma> \<turnstile>\<^sub>d e' : t" using tc_postpend by fastforce
   hence "insert_at 0 t\<^sub>1 \<Gamma> \<turnstile>\<^sub>d incrd 0 e' : t" by simp
-  with subp_cons have "insert_at 0 t\<^sub>1 \<Gamma> \<turnstile>\<^sub>d substd (Suc 0) (incrd 0 e') e : t\<^sub>2" 
+  with tcp_cons have "insert_at 0 t\<^sub>1 \<Gamma> \<turnstile>\<^sub>d substd (Suc 0) (incrd 0 e') e : t\<^sub>2" 
     by (induction \<Gamma>) simp_all
-  with subp_cons obtain ee' where E: "([t\<^sub>1] \<turnstile>\<^sub>d ee' : t\<^sub>2) \<and> 
+  with tcp_cons obtain ee' where E: "([t\<^sub>1] \<turnstile>\<^sub>d ee' : t\<^sub>2) \<and> 
     multisubst es (DLam t\<^sub>1 (substd (Suc 0) (incrd 0 e') e)) = DLam t\<^sub>1 ee' \<and> 
       (\<forall>e\<^sub>2. ([] \<turnstile>\<^sub>d e\<^sub>2 : t\<^sub>1) \<longrightarrow> 
         multisubst (insert_at 0 e\<^sub>2 es) (substd (Suc 0) (incrd 0 e') e) = substd 0 e\<^sub>2 ee')" 
