00Utils/Unification/Substitution.thy
@@ -11,9 +11,6 @@ fun subst :: "subst \<Rightarrow> uexpr \<Rightarrow> uexpr" where
 definition subst_vars :: "subst \<Rightarrow> var set" where
   "subst_vars s = \<Union> (vars ` ran s)"
 
-fun pair_subst :: "subst \<Rightarrow> (uexpr \<times> uexpr) \<Rightarrow> (uexpr \<times> uexpr)" where
-  "pair_subst s (e\<^sub>1, e\<^sub>2) = (subst s e\<^sub>1, subst s e\<^sub>2)"
-
 fun list_subst :: "var \<Rightarrow> uexpr \<Rightarrow> (uexpr \<times> uexpr) list \<Rightarrow> (uexpr \<times> uexpr) list" where
   "list_subst x e' [] = []"
 | "list_subst x e' ((e\<^sub>1, e\<^sub>2) # ess) = (subst [x \<mapsto> e'] e\<^sub>1, subst [x \<mapsto> e'] e\<^sub>2) # list_subst x e' ess"
@@ -117,22 +114,6 @@ lemma list_subst_no_var [simp]: "x \<notin> list_vars ess \<Longrightarrow> list
 
 lemma subst_merge: "subst (extend_subst x e' s) e = subst s (subst [x \<mapsto> e'] e)"
   by (induction e) (simp_all add: extend_subst_def)
-
-lemma [simp]: "pair_subst Map.empty = id"
-proof
-  fix x
-  show "pair_subst Map.empty x = id x" by (cases x) simp_all
-qed
-
-lemma [simp]: "map (pair_subst s) (list_subst x e ess) = 
-    map (pair_subst (extend_subst x e s)) ess"
-  by (induction x e ess rule: list_subst.induct) (simp_all add: subst_merge)
-
-lemma [simp]: "map (pair_subst s) (zip es\<^sub>1 es\<^sub>2) = zip (map (subst s) es\<^sub>1) (map (subst s) es\<^sub>2)"
-proof (induction es\<^sub>1 arbitrary: es\<^sub>2)
-  case (Cons e\<^sub>1 es\<^sub>1)
-  thus ?case by (induction es\<^sub>2) simp_all
-qed simp_all
 
 lemma vars_subst [simp]: "vars (subst s e) \<subseteq> vars e - dom s \<union> subst_vars s"
   and [simp]: "varss (map (subst s) es) \<subseteq> varss es - dom s \<union> subst_vars s"
