Readme.md
@@ -2,11 +2,10 @@ A simple verified compiler, from the (simple typed, call-by-value) lambda calcul
 
 Goals:
 
-Complete missing steps (currently in typechecking)
-Figure out use for other direction of correctness proofs?
-Modularize code with classes
-Remove runtime tags
-Add Parser?
-Add pairs, sums, unit, void, nats, primrec? sructured types?
-Make printing part of the code
-Make initialization part of the code
+- Figure out use for other direction of correctness proofs?
+- Modularize code with classes
+- Remove runtime tags
+- Add Parser?
+- Add pairs, sums, unit, void, nats, primrec? sructured types?
+- Make printing part of the code
+- Make initialization part of the code
